state/Examples.CooperativeMultiThreadingWithIndexT.fst
@@ -26,31 +26,31 @@ instance witnessable_rcontinuation t {| c:witnessable t |} : witnessable (r:ref 
   satisfy = (fun _ pred -> True);
 }
 
-instance targetlang_atree pspec (r:ref int) t {| c:targetlang pspec t |} : targetlang pspec (atree r t) = {
+instance poly_iface_atree pspec (r:ref int) t {| c:poly_iface pspec t |} : poly_iface pspec (atree r t) = {
   wt = witnessable_atree r t #c.wt;
 }
 
-instance targetlang_continuation pspec (r:ref int) t {| c:targetlang pspec t |} : targetlang pspec (continuation r t) = {
+instance poly_iface_continuation pspec (r:ref int) t {| c:poly_iface pspec t |} : poly_iface pspec (continuation r t) = {
   wt = witnessable_continuation r t #c.wt;
 }
 
-instance targetlang_rcontinuation pspec t {| c:targetlang pspec t |} : targetlang pspec (r:ref int -> continuation r t) = {
+instance poly_iface_rcontinuation pspec t {| c:poly_iface pspec t |} : poly_iface pspec (r:ref int -> continuation r t) = {
   wt = witnessable_rcontinuation t #c.wt;
 }
 
 let tgt_typ_run pspec =
-  mk_targetlang_arrow pspec ((int * int) * list (r:(ref int) -> (continuation r unit))) (resexn int)
+  mk_poly_iface_arrow pspec ((int * int) * list (r:(ref int) -> (continuation r unit))) (resexn int)
 
-instance targetlang_run pspec
-  : targetlang pspec (tgt_typ_run pspec) =
-  targetlang_arrow pspec ((int * int) * list (r:(ref int) -> (continuation r unit))) (resexn int)
-    #(targetlang_pair pspec (int * int) (list (r:(ref int) -> (continuation r unit)))
+instance poly_iface_run pspec
+  : poly_iface pspec (tgt_typ_run pspec) =
+  poly_iface_arrow pspec ((int * int) * list (r:(ref int) -> (continuation r unit))) (resexn int)
+    #(poly_iface_pair pspec (int * int) (list (r:(ref int) -> (continuation r unit)))
       #solve
-      #(targetlang_list pspec (r:(ref int) -> (continuation r unit)) #solve))
-    #(targetlang_sum pspec int err #solve #(targetlang_err pspec))
+      #(poly_iface_list pspec (r:(ref int) -> (continuation r unit)) #solve))
+    #(poly_iface_sum pspec int err #solve #(poly_iface_err pspec))
 
-let src_run_type (pspec:targetlang_pspec) =
-  (mk_targetlang_arrow pspec ((nat * int) * l:(list (r:(ref int) -> (continuation r unit))){List.Tot.length l > 0})
+let src_run_type (pspec:poly_iface_pspec) =
+  (mk_poly_iface_arrow pspec ((nat * int) * l:(list (r:(ref int) -> (continuation r unit))){List.Tot.length l > 0})
     #(witnessable_pair (nat * int) (l:(list (r:(ref int) -> (continuation r unit))){List.Tot.length l > 0})
       #(witnessable_pair nat int #(witnessable_refinement int (fun x -> x >= 0))) #solve)
     (resexn int) #solve)
@@ -58,7 +58,7 @@ let src_run_type (pspec:targetlang_pspec) =
 let exportable_run_type (pspec) : exportable_from pspec (src_run_type pspec) Leaf = {
   c_styp = solve;
   ityp = tgt_typ_run pspec;
-  c_ityp = targetlang_run pspec;
+  c_ityp = poly_iface_run pspec;
   export = (fun _ (f:src_run_type pspec) ((fuel, init), tasks) ->
     if fuel >= 0 && List.Tot.Base.length tasks > 0 then
       (f ((fuel, init), tasks))
