state/HigherOrderContracts.fst
@@ -9,14 +9,14 @@ open Witnessable
 open PolyIface
 open SpecTree
 
-instance targetlang_err pspec : targetlang pspec err = {
+instance poly_iface_err pspec : poly_iface pspec err = {
   wt = witnessable_err
 }
 
 class exportable_from pspec (styp: Type u#a) (st:spec_tree pspec) = {
   [@@@no_method] c_styp : witnessable styp;
   [@@@no_method] ityp : Type u#b;
-  [@@@no_method] c_ityp : targetlang pspec ityp;
+  [@@@no_method] c_ityp : poly_iface pspec ityp;
   [@@@no_method] export : hoc_tree st -> styp -> ityp;
   [@@@no_method] lemma_export_preserves_prref :
     x:styp -> prref:mref_pred -> hocs:hoc_tree st -> Lemma (requires (c_styp.satisfy x prref)) (ensures (c_ityp.wt.satisfy (export hocs x) (prref)))
@@ -25,7 +25,7 @@ class exportable_from pspec (styp: Type u#a) (st:spec_tree pspec) = {
 class safe_importable_to pspec (styp: Type u#a) (st:spec_tree pspec) = {
   [@@@no_method] c_styp : witnessable styp;
   [@@@no_method] ityp : Type u#b;
-  [@@@no_method] c_ityp : targetlang pspec ityp;
+  [@@@no_method] c_ityp : poly_iface pspec ityp;
   [@@@no_method] safe_import : ityp -> hoc_tree st -> styp;
   [@@@no_method] lemma_safe_import_preserves_prref :
     x:ityp -> prref:mref_pred -> hocs:hoc_tree st -> Lemma (requires (c_ityp.wt.satisfy x (prref))) (ensures (c_styp.satisfy (safe_import x hocs) (prref)))
@@ -34,14 +34,14 @@ class safe_importable_to pspec (styp: Type u#a) (st:spec_tree pspec) = {
 class importable_to pspec (styp: Type u#a) (st:spec_tree pspec) = {
   [@@@no_method] c_styp : witnessable styp;
   [@@@no_method] ityp : Type u#b;
-  [@@@no_method] c_ityp : targetlang pspec ityp;
+  [@@@no_method] c_ityp : poly_iface pspec ityp;
   [@@@no_method] import : ityp -> hoc_tree st -> resexn styp;
   [@@@no_method] lemma_import_preserves_prref :
     x:ityp -> prref:mref_pred -> hocs:hoc_tree st -> Lemma (requires (c_ityp.wt.satisfy x prref)) (ensures ((witnessable_sum styp err).satisfy (import x hocs) prref))
 }
 
 (** Exportable instances **)
-instance targetlang_is_exportable t pspec {| c1:targetlang pspec t |} : exportable_from pspec t Leaf = {
+instance poly_iface_is_exportable t pspec {| c1:poly_iface pspec t |} : exportable_from pspec t Leaf = {
   c_styp = c1.wt;
   ityp = t;
   c_ityp = solve;
@@ -51,7 +51,7 @@ instance targetlang_is_exportable t pspec {| c1:targetlang pspec t |} : exportab
 instance exportable_unit pspec : exportable_from pspec unit Leaf = {
   c_styp = witnessable_unit;
   ityp = unit;
-  c_ityp = targetlang_unit _;
+  c_ityp = poly_iface_unit _;
   export = (fun Leaf x -> x);
   lemma_export_preserves_prref = (fun _ _ _ -> ())
 }
@@ -59,7 +59,7 @@ instance exportable_unit pspec : exportable_from pspec unit Leaf = {
 instance exportable_err pspec : exportable_from pspec err Leaf = {
   c_styp = witnessable_err;
   ityp = err;
-  c_ityp = targetlang_err _;
+  c_ityp = poly_iface_err _;
   export = (fun Leaf x -> x);
   lemma_export_preserves_prref = (fun _ _ _ -> ())
 }
@@ -67,7 +67,7 @@ instance exportable_err pspec : exportable_from pspec err Leaf = {
 instance exportable_int pspec : exportable_from pspec int Leaf = {
   c_styp = witnessable_int;
   ityp = int;
-  c_ityp = targetlang_int _;
+  c_ityp = poly_iface_int _;
   export = (fun Leaf x -> x);
   lemma_export_preserves_prref = (fun _ _ _ -> ())
 }
@@ -75,7 +75,7 @@ instance exportable_int pspec : exportable_from pspec int Leaf = {
 instance exportable_option pspec t specs {| c:exportable_from pspec t specs |} : exportable_from pspec (option t) specs = {
   c_styp = witnessable_option t #c.c_styp;
   ityp = option c.ityp;
-  c_ityp = targetlang_option _ c.ityp #c.c_ityp;
+  c_ityp = poly_iface_option _ c.ityp #c.c_ityp;
   export = (fun hocs x -> match x with | Some x -> Some (c.export hocs x) | None -> None);
   lemma_export_preserves_prref = (fun x p hocs -> match x with | Some x -> c.lemma_export_preserves_prref x p hocs | None -> ())
 }
@@ -83,7 +83,7 @@ instance exportable_option pspec t specs {| c:exportable_from pspec t specs |} :
 instance exportable_sum pspec t1 t2 s1 s2 {| c1:exportable_from pspec t1 s1 |} {| c2:exportable_from pspec t2 s2 |} : exportable_from pspec (either t1 t2) (EmptyNode s1 s2) = {
   c_styp = witnessable_sum t1 t2 #c1.c_styp #c2.c_styp;
   ityp = either c1.ityp c2.ityp;
-  c_ityp = targetlang_sum _ _ _ #c1.c_ityp #c2.c_ityp;
+  c_ityp = poly_iface_sum _ _ _ #c1.c_ityp #c2.c_ityp;
   export = (fun hocs x -> match x with | Inl x -> Inl (c1.export (left hocs) x) | Inr x -> Inr (c2.export (right hocs) x));
   lemma_export_preserves_prref = (fun x p hocs ->
     match x with | Inl x -> c1.lemma_export_preserves_prref x p (left hocs)| Inr x -> c2.lemma_export_preserves_prref x p (right hocs))
@@ -95,7 +95,7 @@ instance exportable_resexn pspec t spec {| c:exportable_from pspec t spec |} : e
 instance exportable_pair pspec t1 t2 s1 s2 {| c1:exportable_from pspec t1 s1 |} {| c2:exportable_from pspec t2 s2 |} : exportable_from pspec (t1 * t2) (EmptyNode s1 s2) = {
   c_styp = witnessable_pair t1 t2 #c1.c_styp #c2.c_styp;
   ityp = c1.ityp * c2.ityp;
-  c_ityp = targetlang_pair _ _ _ #c1.c_ityp #c2.c_ityp;
+  c_ityp = poly_iface_pair _ _ _ #c1.c_ityp #c2.c_ityp;
   export = (fun hocs (x1, x2) -> (c1.export (left hocs) x1, c2.export (right hocs) x2));
   lemma_export_preserves_prref = (fun (x1, x2) p hocs -> c1.lemma_export_preserves_prref x1 p (left hocs); c2.lemma_export_preserves_prref x2 p (right hocs))
 }
@@ -103,7 +103,7 @@ instance exportable_pair pspec t1 t2 s1 s2 {| c1:exportable_from pspec t1 s1 |} 
 instance exportable_ref pspec t {| c:tc_shareable_type t |} : exportable_from pspec (ref t) Leaf = {
   c_styp = witnessable_mref t _ #solve;
   ityp = ref t;
-  c_ityp = targetlang_ref _ t #c;
+  c_ityp = poly_iface_ref _ t #c;
   export = (fun Leaf x -> x);
   lemma_export_preserves_prref = (fun _ _ _ -> ());
 }
@@ -133,16 +133,16 @@ instance exportable_arrow
   {| c2:exportable_from pspec t2 s2 |}
   (pre:(t1 -> st_pre))
   (post:(x:t1 -> h0:heap -> st_post' (resexn t2) (pre x h0)))
- // (_:squash (forall x h0 r h1. post x h0 r h1 ==> post_targetlang_arrow pspec #(resexn t2) #(witnessable_sum t2 err #c2.c_styp) h0 r h1))
- // (check:select_check pspec t1 unit (pre_targetlang_arrow pspec #_ #c1.c_styp)
+ // (_:squash (forall x h0 r h1. post x h0 r h1 ==> post_poly_iface_arrow pspec #(resexn t2) #(witnessable_sum t2 err #c2.c_styp) h0 r h1))
+ // (check:select_check pspec t1 unit (pre_poly_iface_arrow pspec #_ #c1.c_styp)
  //   (fun x _ _ h1 -> pre x h1))
                 (** ^ the fact that the check has a pre-condition means that the check does not have to enforce it
                       e.g., the invariant on the heap **)
   : exportable_from pspec (x:t1 -> ST (resexn t2) (pre x) (post x))
     (Node (SpecErr true t1 c1.c_styp pre t2 c2.c_styp post) s1 s2) = {
   c_styp = witnessable_arrow t1 (resexn t2) pre post;
-  ityp = mk_targetlang_arrow pspec c1.ityp #c1.c_ityp.wt (resexn c2.ityp) #(witnessable_resexn #c2.ityp #c2.c_ityp.wt);
-  c_ityp = targetlang_arrow pspec c1.ityp (resexn c2.ityp) #c1.c_ityp #(targetlang_sum pspec c2.ityp err #c2.c_ityp) ;
+  ityp = mk_poly_iface_arrow pspec c1.ityp #c1.c_ityp.wt (resexn c2.ityp) #(witnessable_resexn #c2.ityp #c2.c_ityp.wt);
+  c_ityp = poly_iface_arrow pspec c1.ityp (resexn c2.ityp) #c1.c_ityp #(poly_iface_sum pspec c2.ityp err #c2.c_ityp) ;
   export = (fun (hocs:hoc_tree _) (f:(x:t1 -> ST (resexn t2) (pre x) (post x))) (x:c1.ityp) ->
     let Node (| _, myhoc |) lhs rhs : hoc_tree _ = hocs in
     let EnforcePre check c_post = myhoc in
@@ -165,7 +165,7 @@ instance exportable_arrow
 }
 
 (** Importable instances **)
-instance targetlang_is_safely_importable pspec t {| c1:targetlang pspec t |} : safe_importable_to pspec t Leaf = {
+instance poly_iface_is_safely_importable pspec t {| c1:poly_iface pspec t |} : safe_importable_to pspec t Leaf = {
   c_styp = c1.wt;
   ityp = t;
   c_ityp = solve;
@@ -184,7 +184,7 @@ instance safe_importable_is_importable pspec t spec {| c1:safe_importable_to psp
 instance safe_importable_unit pspec : safe_importable_to pspec unit Leaf = {
   c_styp = witnessable_unit;
   ityp = unit;
-  c_ityp = targetlang_unit _;
+  c_ityp = poly_iface_unit _;
   safe_import = (fun x Leaf -> x);
   lemma_safe_import_preserves_prref = (fun _ _ _ -> ())
 }
@@ -192,7 +192,7 @@ instance safe_importable_unit pspec : safe_importable_to pspec unit Leaf = {
 instance safe_importable_err pspec : safe_importable_to pspec err Leaf = {
   c_styp = witnessable_err;
   ityp = err;
-  c_ityp = targetlang_err _;
+  c_ityp = poly_iface_err _;
   safe_import = (fun x Leaf -> x);
   lemma_safe_import_preserves_prref = (fun _ _ _ -> ())
 }
@@ -200,7 +200,7 @@ instance safe_importable_err pspec : safe_importable_to pspec err Leaf = {
 instance importable_option pspec t spec {| c:importable_to pspec t spec |} : importable_to pspec (option t) spec = {
   c_styp = witnessable_option t #c.c_styp;
   ityp = option c.ityp;
-  c_ityp = targetlang_option _ c.ityp #c.c_ityp;
+  c_ityp = poly_iface_option _ c.ityp #c.c_ityp;
   import = (fun x hocs ->
     match x with
     | Some x -> begin
@@ -218,7 +218,7 @@ instance importable_option pspec t spec {| c:importable_to pspec t spec |} : imp
 instance importable_sum pspec t1 t2 s1 s2 {| c1:importable_to pspec t1 s1 |} {| c2:importable_to pspec t2 s2 |} : importable_to pspec (either t1 t2) (EmptyNode s1 s2) = {
   c_styp = witnessable_sum t1 t2 #c1.c_styp #c2.c_styp;
   ityp = either c1.ityp c2.ityp;
-  c_ityp = targetlang_sum _ _ _ #c1.c_ityp #c2.c_ityp;
+  c_ityp = poly_iface_sum _ _ _ #c1.c_ityp #c2.c_ityp;
   import = (fun x hocs ->
     match x with
     | Inl x -> begin
@@ -240,7 +240,7 @@ instance importable_sum pspec t1 t2 s1 s2 {| c1:importable_to pspec t1 s1 |} {| 
 instance importable_pair pspec t1 t2 s1 s2 {| c1:importable_to pspec t1 s1 |} {| c2:importable_to pspec t2 s2 |} : importable_to pspec (t1 * t2) (EmptyNode s1 s2) = {
   c_styp = witnessable_pair t1 t2 #c1.c_styp #c2.c_styp;
   ityp = c1.ityp * c2.ityp;
-  c_ityp = targetlang_pair _ _ _ #c1.c_ityp #c2.c_ityp;
+  c_ityp = poly_iface_pair _ _ _ #c1.c_ityp #c2.c_ityp;
   import = (fun (x, x') hocs ->
     match c1.import x (left hocs) with
     | Inl x -> begin
@@ -257,7 +257,7 @@ instance importable_pair pspec t1 t2 s1 s2 {| c1:importable_to pspec t1 s1 |} {|
 instance safe_importable_ref pspec t {| c:tc_shareable_type t |} : safe_importable_to pspec (ref t) Leaf = {
   c_styp = witnessable_mref t _ #solve;
   ityp = ref t;
-  c_ityp = targetlang_ref _ t;
+  c_ityp = poly_iface_ref _ t;
   safe_import = (fun x Leaf -> x);
   lemma_safe_import_preserves_prref = (fun _ _ _ -> ())
 }
@@ -276,7 +276,7 @@ instance import_refinement pspec t spec {| c:importable_to pspec t spec |} (p:t-
 instance safe_importable_resexn pspec t s {| c:importable_to pspec t s |} : safe_importable_to pspec (resexn t) (EmptyNode s Leaf)= {
   c_styp = witnessable_sum t err #c.c_styp;
   ityp = resexn c.ityp;
-  c_ityp = targetlang_sum _ c.ityp err #c.c_ityp;
+  c_ityp = poly_iface_sum _ c.ityp err #c.c_ityp;
   safe_import = (fun x hocs ->
     match x with
     | Inl x -> begin
@@ -300,14 +300,14 @@ instance safe_importable_arrow
   {| c2:importable_to pspec t2 s2 |}
   (pre:(t1 -> st_pre))
   (post:(x:t1 -> h0:heap -> st_post' (resexn t2) (pre x h0)))
- // (_:squash (forall (x:t1) h0. pre x h0 ==> pre_targetlang_arrow pspec #_ #c1.c_styp x h0))
-//  (_:squash (forall (x:t1) h0 e h1. pre x h0 /\ post_targetlang_arrow pspec #_ #(witnessable_sum t2 err #c2.c_styp) h0 (Inr e) h1 ==> post x h0 (Inr e) h1))
+ // (_:squash (forall (x:t1) h0. pre x h0 ==> pre_poly_iface_arrow pspec #_ #c1.c_styp x h0))
+//  (_:squash (forall (x:t1) h0 e h1. pre x h0 /\ post_poly_iface_arrow pspec #_ #(witnessable_sum t2 err #c2.c_styp) h0 (Inr e) h1 ==> post x h0 (Inr e) h1))
 //  (capture_check:select_check pspec t1 (resexn t2) #(witnessable_sum _ err #c2.c_styp) pre post)
   : safe_importable_to pspec (x:t1 -> ST (resexn t2) (pre x) (post x)) (Node (SpecErr false t1 c1.c_styp pre t2 c2.c_styp post) s1 s2) = {
   c_styp = witnessable_arrow t1 (resexn t2) pre post;
-  ityp = mk_targetlang_arrow pspec c1.ityp #c1.c_ityp.wt (resexn c2.ityp) #(witnessable_resexn #c2.ityp #c2.c_ityp.wt);
-  c_ityp = targetlang_arrow _ c1.ityp (resexn c2.ityp) #_ #(targetlang_sum _ c2.ityp err #c2.c_ityp);
-  safe_import = (fun (f:mk_targetlang_arrow pspec c1.ityp #c1.c_ityp.wt (resexn c2.ityp) #(witnessable_sum c2.ityp err #c2.c_ityp.wt)) (hocs:hoc_tree _) (x:t1) ->
+  ityp = mk_poly_iface_arrow pspec c1.ityp #c1.c_ityp.wt (resexn c2.ityp) #(witnessable_resexn #c2.ityp #c2.c_ityp.wt);
+  c_ityp = poly_iface_arrow _ c1.ityp (resexn c2.ityp) #_ #(poly_iface_sum _ c2.ityp err #c2.c_ityp);
+  safe_import = (fun (f:mk_poly_iface_arrow pspec c1.ityp #c1.c_ityp.wt (resexn c2.ityp) #(witnessable_sum c2.ityp err #c2.c_ityp.wt)) (hocs:hoc_tree _) (x:t1) ->
     let Node (| _, myhoc |) lhs rhs : hoc_tree _ = hocs in
     let EnforcePost c_pre c_post check = myhoc in
     c_pre x;
@@ -332,13 +332,13 @@ instance safe_importable_arrow_safe
   {| c2:safe_importable_to pspec t2 s2 |}
   (pre:(t1 -> st_pre))
   (post:(x:t1 -> h0:heap -> st_post' t2 (pre x h0)))
- // (_:squash (forall (x:t1) h0. pre x h0 ==> pre_targetlang_arrow pspec #_ #c1.c_styp x h0))
-//  (_:squash (forall (x:t1) h0 r h1. pre x h0 /\ post_targetlang_arrow pspec #_ #c2.c_styp h0 r h1 ==> post x h0 r h1))
+ // (_:squash (forall (x:t1) h0. pre x h0 ==> pre_poly_iface_arrow pspec #_ #c1.c_styp x h0))
+//  (_:squash (forall (x:t1) h0 r h1. pre x h0 /\ post_poly_iface_arrow pspec #_ #c2.c_styp h0 r h1 ==> post x h0 r h1))
   : safe_importable_to pspec (x:t1 -> ST t2 (pre x) (post x)) (Node (Spec false t1 c1.c_styp pre t2 c2.c_styp post) s1 s2) = {
   c_styp = witnessable_arrow t1 t2 pre post;
-  ityp = mk_targetlang_arrow pspec c1.ityp #c1.c_ityp.wt c2.ityp #c2.c_ityp.wt;
-  c_ityp = targetlang_arrow _ c1.ityp c2.ityp #_ #c2.c_ityp;
-  safe_import = (fun (f:mk_targetlang_arrow pspec c1.ityp #c1.c_ityp.wt c2.ityp #c2.c_ityp.wt) hocs (x:t1) ->
+  ityp = mk_poly_iface_arrow pspec c1.ityp #c1.c_ityp.wt c2.ityp #c2.c_ityp.wt;
+  c_ityp = poly_iface_arrow _ c1.ityp c2.ityp #_ #c2.c_ityp;
+  safe_import = (fun (f:mk_poly_iface_arrow pspec c1.ityp #c1.c_ityp.wt c2.ityp #c2.c_ityp.wt) hocs (x:t1) ->
     let Node (| _, myhoc |) lhs rhs : hoc_tree _ = hocs in
     let TrivialPost c_pre c_post = myhoc in
     c_pre x;
@@ -428,7 +428,7 @@ let f_xeq5_hoc : hoc concrete_spec f_xeq5_spec =
     (fun rx ->
       let rx :ref int = rx in
       let eh0 = get_heap () in
-      let check : cb_check concrete_spec (ref int) _ (pre_targetlang_arrow concrete_spec #(SpecErr?.argt f_xeq5_spec) #(SpecErr?.wt_argt f_xeq5_spec)) (fun x _ _ h1 -> (SpecErr?.pre f_xeq5_spec) x h1) rx eh0 =
+      let check : cb_check concrete_spec (ref int) _ (pre_poly_iface_arrow concrete_spec #(SpecErr?.argt f_xeq5_spec) #(SpecErr?.wt_argt f_xeq5_spec)) (fun x _ _ h1 -> (SpecErr?.pre f_xeq5_spec) x h1) rx eh0 =
         (fun _ ->
           recall (contains_pred rx);
           if 5 = sst_read rx then Inl () else Inr (Contract_failure "x has changed")) in
